Remove the abstraction from the core STLC; we'll define Pact directly

src/Eval.v
@@ -4,8 +4,7 @@ Require Import
   Ty
   Exp
   Sub
-  Sem
-  Lang.
+  Sem.
 
 From Equations Require Import Equations.
 Set Equations With UIP.
@@ -16,30 +15,21 @@ Import ListNotations.
 
 Section Eval.
 
-Context {t : Type}.
-Context {x : Env t → Ty t → Type}.
-Context `{Lang t x}.
-
-Inductive Eval : ∀ {τ}, Exp t x [] τ → Exp t x [] τ → Prop :=
-  | EvTerm t1 (e1 : x [] t1) (e2 : Exp t x [] t1) :
-    eval e1 e2 →
-    Eval (TERM e1) e2
-
-  | EvLam t1 t2 (e : Exp t x [t1] t2) :
+Inductive Eval : ∀ {τ}, Exp [] τ → Exp [] τ → Prop :=
+  | EvLam t1 t2 (e : Exp [t1] t2) :
     Eval (LAM e) (LAM e)
 
-  | EvApp t1 t2 e v w (e1 : Exp t x [] (t1 ⟶ t2)) e2 :
+  | EvApp t1 t2 e v w (e1 : Exp [] (t1 ⟶ t2)) e2 :
     Eval e1 (LAM e) →
     Eval e2 w →
-    Eval (STmExp (ren:=@ren _ _ _) (sub:=@sub _ _ _) {| w |} e) v →
+    Eval (STmExp {| w |} e) v →
     Eval (APP e1 e2) v.
 
-Theorem soundness τ (e : Exp t x [] τ) v :
-  Eval e v → SemExp SemT (@SemX _ _ _) e = SemExp SemT (@SemX _ _ _) v.
+Theorem soundness τ (e : Exp [] τ) v :
+  Eval e v → SemExp e = SemExp v.
 Proof.
   intros.
-  induction H0; simpl; auto.
-  - now apply (eval_sound _ e1 e2).
+  induction H; simpl; auto.
   - extensionality E.
     destruct E.
     rewrite IHEval1.
@@ -50,8 +40,6 @@ Proof.
     + simpl.
       unfold hdSub.
       now rewrite consSub_equation_1.
-    + now intros; apply SemX_SemRen.
-    + now intros; apply SemX_SemSub.
 Qed.
 
 End Eval.
