src/Exp.v
@@ -10,32 +10,28 @@ Import ListNotations.
 
 Section Exp.
 
-Variable t : Type.
+Definition Env := list Ty.
 
-Definition Env := list (Ty t).
-
-Inductive Var : Env → Ty t → Type :=
+Inductive Var : Env → Ty → Type :=
   | ZV Γ τ    : Var (τ :: Γ) τ
   | SV Γ τ τ' : Var Γ τ → Var (τ' :: Γ) τ.
 
 Derive Signature NoConfusion for Var.
 
-Variable x : Env → Ty t → Type.
-
-Inductive Exp Γ : Ty t → Type :=
-  | TERM {τ}      : x Γ τ → Exp Γ τ
+Inductive Exp Γ : Ty → Type :=
   | VAR {τ}       : Var Γ τ → Exp Γ τ
   | LAM {dom cod} : Exp (dom :: Γ) cod → Exp Γ (dom ⟶ cod)
-  | APP {dom cod} : Exp Γ (dom ⟶ cod) → Exp Γ dom → Exp Γ cod.
+  | APP {dom cod} : Exp Γ (dom ⟶ cod) → Exp Γ dom → Exp Γ cod
+
+  .
 
 Derive Signature for Exp.
 
 End Exp.
 
-Arguments ZV {_ _ _}.
-Arguments SV {_ _ _ _} _.
+Arguments ZV {_ _}.
+Arguments SV {_ _ _} _.
 
-Arguments TERM {t x Γ τ} _.
-Arguments VAR {t x Γ τ} _.
-Arguments LAM {t x Γ dom cod} _.
-Arguments APP {t x Γ dom cod} _ _.
+Arguments VAR {Γ τ} _.
+Arguments LAM {Γ dom cod} _.
+Arguments APP {Γ dom cod} _ _.
