src/Sem.v
@@ -16,12 +16,8 @@ Import ListNotations.
 
 Section Sem.
 
-Context {t : Type}.
-Variable SemT : t → Type.
-
-Fixpoint SemTy (τ : Ty t) : Type :=
+Fixpoint SemTy (τ : Ty) : Type :=
   match τ with
-  | TYP y => SemT y
   | TARR dom cod => SemTy dom → SemTy cod
   end.
 
@@ -35,7 +31,7 @@ Equations trunc {Γ} Γ' `(E : SemEnv (Γ' ++ Γ)) : SemEnv Γ :=
   trunc []        E := E;
   trunc (x :: xs) E := trunc xs (snd E).
 
-Fixpoint SemVar `(v : Var t Γ τ) : SemEnv Γ → SemTy τ :=
+Fixpoint SemVar `(v : Var Γ τ) : SemEnv Γ → SemTy τ :=
   match v with
   | ZV   => λ se, fst se
   | SV v => λ se, SemVar v (snd se)
@@ -47,7 +43,7 @@ Fixpoint SemRen {Γ Γ'} : Ren Γ' Γ → SemEnv Γ → SemEnv Γ' :=
   | _ :: _ => λ r se, (SemVar (hdRen r) se, SemRen (tlRen r) se)
   end.
 
-Lemma SemRenVarComm Γ τ (v : Var t Γ τ) Γ' (r : Ren Γ Γ') :
+Lemma SemRenVarComm Γ τ (v : Var Γ τ) Γ' (r : Ren Γ Γ') :
   ∀ se, SemVar v (SemRen r se) = SemVar (r _ v) se.
 Proof.
   intros.
@@ -137,7 +133,7 @@ Proof.
     rewrite trunc_equation_2.
     rewrite <- IHΓ.
     replace (λ τ v,
-              @SV t (Γ ++ Γ') τ a (@skipn t Γ' Γ τ v))
+              @SV (Γ ++ Γ') τ a (@skipn Γ' Γ τ v))
        with (RcR (Γ:=Γ') (skip1 (τ:=a)) (skipn Γ))
          by reflexivity.
     rewrite SemRen_RcR.
@@ -152,15 +148,8 @@ Corollary SemRen_SV `(E : SemEnv Γ) `(x : SemTy τ) :
   SemRen (λ _, SV) (x, E) = E.
 Proof. now rewrite SemRen_SV_snd. Qed.
 
-Context {x : Env t → Ty t → Type}.
-
-Variable SemX : ∀ Γ (τ : Ty t), x Γ τ → SemEnv Γ → SemTy τ.
-
-Context {ren : ∀ Γ Γ' τ, Ren Γ Γ' → x Γ τ → x Γ' τ}.
-
-Fixpoint SemExp `(e : Exp t x Γ τ) : SemEnv Γ → SemTy τ :=
+Fixpoint SemExp `(e : Exp Γ τ) : SemEnv Γ → SemTy τ :=
   match e with
-  | TERM r    => SemX _ _ r
   | VAR v     => SemVar v
   | LAM e     => λ se, λ x, SemExp e (x, se)
   | APP e1 e2 => λ se, SemExp e1 se (SemExp e2 se)
@@ -172,18 +161,12 @@ Fixpoint SemSub {Γ Γ'} : Sub Γ' Γ → SemEnv Γ → SemEnv Γ' :=
   | _ :: _ => λ s se, (SemExp (hdSub s) se, SemSub (tlSub s) se)
   end.
 
-Context {sub : ∀ Γ Γ' τ, Sub (x:=x) Γ Γ' → x Γ τ → x Γ' τ}.
-
-Hypothesis SemX_SemRen : ∀ Γ Γ' τ z r E,
-  SemX Γ τ z (SemRen r E) = SemX Γ' τ (ren _ _ _ r z) E.
-
-Lemma SemRenComm Γ τ (e : Exp t x Γ τ) Γ' (r : Ren Γ Γ') :
-  ∀ se, SemExp e (SemRen r se) = SemExp (RTmExp (ren:=ren) r e) se.
+Lemma SemRenComm Γ τ (e : Exp Γ τ) Γ' (r : Ren Γ Γ') :
+  ∀ se, SemExp e (SemRen r se) = SemExp (RTmExp r e) se.
 Proof.
   intros.
   generalize dependent Γ'.
   induction e; simpl; intros.
-  - now apply SemX_SemRen.
   - induction v; simpl.
     + reflexivity.
     + now rewrite IHv.
@@ -203,8 +186,8 @@ Proof.
 Qed.
 
 Lemma SemExp_wk `(E : SemEnv Γ)
-      {τ τ'} (y : SemTy τ') (e : Exp t x Γ τ) :
-  SemExp (wk (ren:=ren) e) (y, E) = SemExp e E.
+      {τ τ'} (y : SemTy τ') (e : Exp Γ τ) :
+  SemExp (wk e) (y, E) = SemExp e E.
 Proof.
   unfold wk.
   rewrite <- SemRenComm; simpl.
@@ -212,16 +195,12 @@ Proof.
   now eapply SemRen_SV; eauto.
 Qed.
 
-Hypothesis SemX_SemSub : ∀ Γ Γ' τ z s E,
-  SemX Γ τ z (SemSub s E) = SemX Γ' τ (sub _ _ _ s z) E.
-
-Lemma SemSubComm Γ τ (e : Exp t x Γ τ) Γ' (s : Sub Γ Γ') :
-  ∀ se, SemExp e (SemSub s se) = SemExp (STmExp (ren:=ren) (sub:=sub) s e) se.
+Lemma SemSubComm Γ τ (e : Exp Γ τ) Γ' (s : Sub Γ Γ') :
+  ∀ se, SemExp e (SemSub s se) = SemExp (STmExp s e) se.
 Proof.
   intros.
   generalize dependent Γ'.
   induction e; simpl; intros.
-  - now apply SemX_SemSub.
   - induction v; simpl.
     + reflexivity.
     + now rewrite IHv.
@@ -230,13 +209,13 @@ Proof.
     rewrite <- IHe; clear IHe.
     simpl.
     f_equal.
-    clear -SemX_SemRen.
+    clear.
     f_equal.
     unfold tlSub.
     induction Γ; simpl; auto.
     f_equal.
     + unfold hdSub.
-      clear -SemX_SemRen.
+      clear.
       rewrite STmL_equation_2.
       now rewrite SemExp_wk.
     + unfold tlSub.
@@ -250,8 +229,8 @@ Lemma SemExp_identity `(E : SemEnv Γ) τ :
 Proof. now extensionality z. Qed.
 
 Lemma SemExp_compose `(E : SemEnv Γ)
-      {τ τ' τ''} (f : Exp t x Γ (τ' ⟶ τ'')) (g : Exp t x Γ (τ ⟶ τ')) :
-  SemExp (compose (ren:=ren) f g) E = SemExp f E ∘ SemExp g E.
+      {τ τ' τ''} (f : Exp Γ (τ' ⟶ τ'')) (g : Exp Γ (τ ⟶ τ')) :
+  SemExp (compose f g) E = SemExp f E ∘ SemExp g E.
 Proof.
   extensionality z.
   fold SemTy in z.
@@ -260,16 +239,16 @@ Proof.
 Qed.
 
 Lemma SemExp_compose_identity_right `(E : SemEnv Γ)
-      {τ τ'} (f : Exp t x Γ (τ ⟶ τ')) :
-  SemExp (compose (ren:=ren) f (identity Γ τ)) E = SemExp f E.
+      {τ τ'} (f : Exp Γ (τ ⟶ τ')) :
+  SemExp (compose f (identity Γ τ)) E = SemExp f E.
 Proof.
   rewrite SemExp_compose.
   reflexivity.
 Qed.
 
 Lemma SemExp_compose_identity_left `(E : SemEnv Γ)
-      {τ τ'} (f : Exp t x Γ (τ ⟶ τ')) :
-  SemExp (compose (ren:=ren) (identity Γ τ') f) E = SemExp f E.
+      {τ τ'} (f : Exp Γ (τ ⟶ τ')) :
+  SemExp (compose (identity Γ τ') f) E = SemExp f E.
 Proof.
   rewrite SemExp_compose.
   reflexivity.
@@ -277,11 +256,11 @@ Qed.
 
 Lemma SemExp_compose_assoc `(E : SemEnv Γ)
       {τ τ' τ'' τ'''}
-      (f : Exp t x Γ (τ'' ⟶ τ'''))
-      (g : Exp t x Γ (τ' ⟶ τ''))
-      (h : Exp t x Γ (τ ⟶ τ')) :
-  SemExp (compose (ren:=ren) f (compose (ren:=ren) g h)) E =
-  SemExp (compose (ren:=ren) (compose (ren:=ren) f g) h) E.
+      (f : Exp Γ (τ'' ⟶ τ'''))
+      (g : Exp Γ (τ' ⟶ τ''))
+      (h : Exp Γ (τ ⟶ τ')) :
+  SemExp (compose f (compose g h)) E =
+  SemExp (compose (compose f g) h) E.
 Proof.
   rewrite !SemExp_compose.
   now rewrite compose_assoc.
