src/Sub.v
@@ -14,36 +14,28 @@ Import ListNotations.
 
 Section Sub.
 
-Context {t : Type}.
-Context {x : Env t → Ty t → Type}.
+Definition Sub Γ Γ' := ∀ τ, Var Γ τ → Exp Γ' τ.
 
-Definition Sub Γ Γ' := ∀ τ, Var t Γ τ → Exp t x Γ' τ.
+Definition idSub {Γ} : Sub Γ Γ := @VAR Γ.
 
-Definition idSub {Γ} : Sub Γ Γ := @VAR t x Γ.
-
-Equations consSub {Γ Γ' τ} (e : Exp t x Γ' τ) (s : Sub Γ Γ')
+Equations consSub {Γ Γ' τ} (e : Exp Γ' τ) (s : Sub Γ Γ')
           (* Sub (τ :: Γ) Γ' *)
-          τ' (v : Var t (τ :: Γ) τ') : Exp t x Γ' τ' :=
+          τ' (v : Var (τ :: Γ) τ') : Exp Γ' τ' :=
   consSub e s τ' ZV      := e;
   consSub e s τ' (SV v') := s _ v'.
 
 Definition tlSub {Γ Γ' τ} (s : Sub (τ :: Γ) Γ') : Sub Γ Γ' :=
   fun τ' v => s τ' (SV v).
-Definition hdSub {Γ Γ' τ} (s : Sub (τ :: Γ) Γ') : Exp t x Γ' τ := s τ ZV.
-
-Context {ren : ∀ Γ Γ' τ, Ren Γ Γ' → x Γ τ → x Γ' τ}.
+Definition hdSub {Γ Γ' τ} (s : Sub (τ :: Γ) Γ') : Exp Γ' τ := s τ ZV.
 
 Equations STmL {Γ Γ' τ} (s : Sub Γ Γ')
           (* Sub (τ :: Γ) (τ :: Γ') *)
-          τ' (v : Var t (τ :: Γ) τ') : Exp t x (τ :: Γ') τ' :=
+          τ' (v : Var (τ :: Γ) τ') : Exp (τ :: Γ') τ' :=
   STmL _ τ' ZV      := VAR ZV;
   STmL _ τ' (SV v') := wk (s _ v').
 
-Context {sub : ∀ Γ Γ' τ, Sub Γ Γ' → x Γ τ → x Γ' τ}.
-
-Fixpoint STmExp {Γ Γ' τ} (s : Sub Γ Γ') (e : Exp t x Γ τ) : Exp t x Γ' τ :=
+Fixpoint STmExp {Γ Γ' τ} (s : Sub Γ Γ') (e : Exp Γ τ) : Exp Γ' τ :=
   match e with
-  | TERM z    => TERM (sub _ _ _ s z)
   | VAR v     => s _ v
   | APP e1 e2 => APP (STmExp s e1) (STmExp s e2)
   | LAM e     => LAM (STmExp (STmL s) e)
@@ -53,7 +45,7 @@ Definition ScR {Γ Γ' Γ''} (s : Sub Γ' Γ'') (r : Ren Γ Γ') :=
   (λ τ v, s τ (r τ v)) : Sub Γ Γ''.
 
 Definition RcS {Γ Γ' Γ''} (r : Ren Γ' Γ'') (s : Sub Γ Γ') :=
-  (λ τ v, RTmExp (ren:=ren) r (s τ v)) : Sub Γ Γ''.
+  (λ τ v, RTmExp r (s τ v)) : Sub Γ Γ''.
 
 Definition ScS {Γ Γ' Γ''} (s : Sub Γ' Γ'') (s' : Sub Γ Γ') :=
   (λ τ v, STmExp s (s' τ v)) : Sub Γ Γ''.
