src/Ty.v
@@ -6,17 +6,15 @@ Set Equations With UIP.
 
 Section Ty.
 
-Variable t : Type.
-
 Inductive Ty : Type :=
-  | TYP : t → Ty
-  | TARR : Ty → Ty → Ty.
+  | TARR : Ty → Ty → Ty
 
-Derive NoConfusion Subterm for Ty.
+  .
+
+Derive NoConfusion for Ty.
 
 End Ty.
 
-Arguments TYP {t} _.
-Arguments TARR {t} _ _.
+Arguments TARR _ _.
 
 Infix "⟶" := TARR (at level 30, right associativity).
